\chapter{Rings and modules}
\label{ch:rings}

\section{Rings and homomorphisms}

\begin{definition}
    A \emph{ring} is a triple \((R, +, \cdot)\), where \(R\) is a nonempty set
    and \(+\) and \(\cdot\) are two binary operations (often referred to as
    `addition' and `multiplication', respectively) such that:
    \begin{enumerate}[label=(\alph*)]
        \item \((R, +)\) is an abelian group.
        \item Multiplication is associative, i.e. \((a \cdot b) \cdot c = a
        \cdot (b \cdot c)\) for all \(a, b, c \in R\).
        \item Multiplication is distributive over addition, i.e. \(a \cdot (b +
        c) = a \cdot b + a \cdot c\) and \((a + b) \cdot c = a \cdot c + b \cdot
        c\) for all \(a, b, c \in R\).
        \item There exists a distinguished element \(1 \in R\) such that \(1
        \cdot a = a \cdot 1 = a\) for all \(a \in R\).
    \end{enumerate}
\end{definition}

More succinctly, axioms (b) and (d) above tell us that \((R, \cdot)\) is a
monoid with identity element \(1\).

Some texts may refer to the triple \((R, +, \cdot)\) satisfying the above axioms
as a \emph{ring with unity} or a \emph{ring with \(1\)} and only require that
the first three axioms be satisfied for \((R, +, \cdot)\) to be a ring. Rings
without unity are sometimes referred to as \emph{rngs} in the literature. For
example, the set of even integers \(2\Z\) with the usual operations of addition
and multiplication satisfies all the axioms above except for the requirement
that the multiplicative identity \(1\) be in \(2\Z\). Thus it is a `rng' by the
preceding definition. Nevertheless, we shall follow the above definition in this
text and all rings will be assumed to have a multiplicative identity unless
otherwise stated. If multiplication is commutative, i.e. \(a \cdot b = b \cdot
a\) for all \(a, b \in R\), then we say that \(R\) is a \emph{commutative ring}.
As in Chapter~\ref{ch:groups}, we will often write \(ab\) instead of \(a \cdot
b\).

Some elementary properties of rings derive from the properties of additive
groups and monoids. The identity element of the abelian group \((R, +)\) is
often denoted by \(0\), and is called the \emph{zero} of the ring \(R\). Since
\(R\) is an abelian group under addition, it follows that \(0\) must be unique,
as is the additive inverse \(-a\) of every element \(a \in R\). Moreover, for
all \(a, b \in R\), we have
\[
    -(-a) = a, \quad -0 = 0, \quad \text{and} \quad -(a + b) = (-a) + (-b).
\]
The usual laws for multiples of the form \(na\) where \(a \in R\) and \(n\) is
an integer also hold in rings. To wit, we have
\[
    (m+n)a = ma + na, \quad (-m)a = -(ma), \quad \text{and} \quad m(na) = (mn)a
\]
and because \(R\) is also abelian we have
\[
    m(a+b) = ma + mb
\]
for all \(a, b \in R\) and \(m, n \in \mathbb{Z}\). Because \(R\) is also a
monoid under multiplication, the distinguished element \(1 \in R\) (called the
\emph{unity}) must likewise be unique and the usual laws of exponents must
similarly hold, so that we have, for all \(a \in R\) and \(m, n \in
\mathbb{Z}\),
\[
    a^m a^n = a^{m+n} \quad \text{and} \quad (a^m)^n = a^{mn}.
\]

Other properties do not directly derive from \(R\) being an abelian group or a
monoid under addition and multiplication, respectively, but are consequences of
the distributive law. In particular we have the following results.

\begin{theorem}
    Let \(R\) be a ring. Then
    \begin{enumerate}[label={\normalfont(\alph*)}]
        \item \(0a = a0 = 0\) for all \(a \in R\);
        \item if \(R\) is not the zero ring, then \(0 \neq 1\);
        \item \((-a)b = a(-b) = -(ab)\) for all \(a, b \in R\);
        \item For all \(a, b \in R\),
        \[
            \left(\sum_{i=1}^{m} a_i\right)\left(\sum_{j=1}^{n} b_j\right) = \sum_{i=1}^{m} \sum_{j=1}^{n} a_i b_j;
        \]
        \item \((na)b = n(ab) = a(nb)\) for all \(a, b \in R\) and \(n \in
        \mathbb{Z}\).
    \end{enumerate}
\end{theorem}

\begin{proof}\(\)
    \begin{enumerate}[label=(\alph*), wide]
        \item Since \(0\) is the additive identity, we have \(0a = (0 + 0)a = 0a
        + 0a\), whence \(0a = 0\). Similarly, \(a0 = a(0 + 0) = a0 + a0\), so
        \(a0 = 0\).

        \item If \(0 = 1\), then for all \(a \in R\), we have \(a = a1 = a0 = 0\), from which it follows that \(R\) contains only the zero element, i.e., \(R\) is the zero ring.
        
        \item From (a) above and the distributive law, we have
        \[
            0 = 0b = (a + (-a))b = ab + (-a)b,
        \]
        whence \((-a)b = -(ab)\). An analogous argument shows that \(a(-b) = -(ab)\).

        Since \(-(-a) = a\), we then have, as an immediate consequence, that \((-a)(-b) = a(-(-b)) = a(b) = ab\) and in particular \((-1)(-1) = 1\) and \((-1)a = -a\).

        \item For \(m = 1\), the proof is by induction on \(n\), with the case \(n = 2\) being left distribution. Having established this rule for \(m = 1\), a second induction on \(m\) completes the proof.
        
        \item For positive \(n\), the first equation is given by \(ab + \cdots + ab = (a + \cdots + a)b\) and is thus a special case of (d) above. For negative \(n\), we can use the result in (c).
    \end{enumerate}
\end{proof}


\begin{definition}
    \label{def:ring-homomorphism}
    A \emph{homomorphism of rings} is a (set) function \(\phi: R \to S\) between
    two rings \(R\) and \(S\) such that for all \(a, b \in R\),
    \begin{enumerate}[label=(\alph*)]
        \item \(\phi(a + b) = \phi(a) + \phi(b)\);
        \item \(\phi(ab) = \phi(a)\phi(b)\);
        \item \(\phi(1) = 1'\).
    \end{enumerate}
    Here the addition and multiplication on the left-hand side are those of
    \(R\), while the addition and multiplication on the right-hand side are
    those of \(S\); the unity of \(R\) is denoted by \(1\) and the unity of
    \(S\) is denoted by \(1'\).
\end{definition}

From the definition it then follows that \(\phi\) is a homomorphism of the additive groups \(R\) and \(S\) so that \(\phi(0) = 0\) and \(\phi(-a) = -\phi(a)\) for all \(a \in R\). However, as part of our definition of a ring homomorphism, we require that \(\phi(1) = 1'\) so that \(\phi\) is also a homomorphism of the monoids \((R, \cdot)\) and \((S, \cdot)\). Indeed the condition \(\phi(1) = 1'\) does not directly follow from (a) and (b) in Definition~\ref{def:ring-homomorphism}. For example, consider a commutative ring \(R\) that contains an idempoent element \(e\), i.e., an element \(e\) satisfying \(e^2 = e\). Then the function \(\phi: R \to R\) defined by \(x \mapsto xe\) satisfies conditions (a) and (b) above, viz., \[\phi(x + y) = (x + y)e = xe + ye = \phi(x) + \phi(y);\] we also have \(\phi(x) \phi(y) = (xe)(ye) = (xy)e\) because \(R\) is commutative and \(e\) is idempotent and thus \(\phi(xy) = \phi(x) \phi(y)\). However, \(\phi(1) = 1e = e\) and thus condition (c) is not satisfied.